\section{三角函数相关公式}

\begin{spacing}{\hangju}
    \begin{multicols}{2}
        \noindent $\displaystyle \sin{2x}=2\sin{x}\cos{x}$

        \noindent $\displaystyle \sin{3x}=-4\sin^3{x}+3\sin{x}$

        \noindent $\displaystyle \cos{3x}=4\cos^3{x}-3\cos{x}$

        \noindent $\displaystyle \tan{2x}=\frac{2\tan{x}}{1-\tan^2{x}}$

        \noindent $\displaystyle \cot{2x}=\frac{\cot^2{x}-1}{2\cot{x}}$

        \noindent $\displaystyle \sin^2{\frac{x}{2}}=\frac{1}{2}(1-\cos{x})$

        \noindent $\displaystyle \cos^2{\frac{x}{2}}=\frac{1}{2}(1+\cos{x})$

        \noindent $\displaystyle \sin^2{x}=\frac{1}{2}(1-\cos{2x})$

        \noindent $\displaystyle \sin{\frac{x}{2}}=\pm\sqrt{\frac{1-\cos{x}}{2}}$

        \noindent $\displaystyle \cos{\frac{x}{2}}=\pm\sqrt{\frac{1+\cos{x}}{2}}$

        \noindent $\displaystyle \sin{\alpha}+\sin{\beta}=2\sin{\frac{\alpha+\beta}{2}}\cos{\frac{\alpha-\beta}{2}}$

        \noindent $\displaystyle \sin{\alpha}-\sin{\beta}=2\sin{\frac{\alpha-\beta}{2}}\cos{\frac{\alpha+\beta}{2}}$

        \noindent $\displaystyle \cos{\alpha} + \cos{\beta} = 2\cos{\frac{\alpha+\beta}{2}}\cos{\frac{\alpha-\beta}{2}}$

        \noindent $\cos{\alpha} - \cos{\beta} = -2\sin{\frac{\alpha+\beta}{2}}\cos{\frac{\alpha-\beta}{2}}$

        \noindent $\displaystyle \sin{(\alpha \pm \beta)}=\sin{\alpha}\cos{\beta} \pm \cos{\alpha}\sin{\beta}$

        \noindent $\displaystyle \cos{(\alpha \pm \beta)}=\cos{\alpha}\cos{\beta} \mp \sin{\alpha}\sin{\beta}$

        \noindent $\displaystyle \tan{(\alpha \pm \beta)}=\frac{\tan{\alpha} \pm \tan{\beta}}{1 \mp \tan{\alpha}\tan{\beta}}$

        \noindent $\displaystyle \cot{(\alpha \pm \beta)}=\frac{\cot{\alpha}\cot{\beta} \mp 1}{\cot{\beta} \pm \cot{\alpha}}$

    \end{multicols}

    \noindent $\displaystyle \tan{ \frac{x}{2} } = \frac{ 1-\cos{x} }{ \sin{x} }=\frac{\sin{x}}{1+\cos{x}} = \pm \sqrt{\frac{1 - \cos{x}}{1 + \cos{x}}}$

    \noindent $\displaystyle \cot{\frac{x}{2}} = \frac{\sin{x}}{1-\cos{x}} = \frac{1+\cos{x}}{\sin{x}} = \pm \sqrt{\frac{1 + \cos{x}}{1 - \cos{x}}}$

    \noindent $\cos{2x}=\cos^2{x}-\sin^2{x}=1-2\sin^2{x}=2\cos^2{x}-1$

    \noindent $\sin{\alpha}\cos{\beta}=\frac{1}{2}[\sin{(\alpha+\beta)}+\sin{(\alpha-\beta)}]$

    \noindent $\cos{\alpha}\sin{\beta} = \frac{1}{2} [\sin{(\alpha+\beta)} - \sin{(\alpha-\beta)}]$

    \noindent $\cos{\alpha}\cos{\beta}=\frac{1}{2}[\cos{(\alpha+\beta)}+\cos{(\alpha-\beta)}]$

    \noindent $\sin{\alpha}\sin{\beta} =
        \frac{1}{2}[\cos{(\alpha-\beta)}-\cos{(\alpha+\beta)}]$

    \noindent 万能公式：若$u=\tan{\frac{x}{2}}(-\pi<x<\pi)$，则
        $\sin{x}=\frac{2u}{1+u^2}, \cos{x}=\frac{1-u^2}{1+u^2}$

\end{spacing}